Cslib/Computability/LambdaCalculus/Untyped/LocallyNameless/Properties.lean
@@ -6,12 +6,12 @@ Authors: Chris Henson
 
 import Cslib.Computability.LambdaCalculus.Untyped.LocallyNameless.Basic
 
-variable {Fvar : Type}
+variable {Var : Type}
 
 namespace LambdaCalculus.LocallyNameless.Term
 
 /-- An opening appearing in both sides of an equality of terms can be removed. -/
-lemma open_lc_aux (e : Term Fvar) : ∀ (j v i u),
+lemma open_lc_aux (e : Term Var) : ∀ (j v i u),
   i ≠ j ->
   e ⟦j ↝ v⟧ = (e ⟦j ↝ v⟧) ⟦i ↝ u⟧ ->
   e = e ⟦i ↝ u⟧ := by
@@ -23,7 +23,7 @@ lemma open_lc_aux (e : Term Fvar) : ∀ (j v i u),
   case lam ih => exact ih (j+1) v (i+1) u (by aesop) h
 
 /-- Opening is associative for nonclashing free variables. -/
-lemma swap_open_fvars (k n : ℕ) (x y : Fvar) (m : Term Fvar) : 
+lemma swap_open_fvars (k n : ℕ) (x y : Var) (m : Term Var) : 
     k ≠ n → x ≠ y → m⟦n ↝ fvar y⟧⟦k ↝ fvar x⟧ = m⟦k ↝ fvar x⟧⟦n ↝ fvar y⟧ := by
   revert k n
   induction' m <;> intros k n ne_kn ne_xy <;> simp
@@ -31,14 +31,14 @@ lemma swap_open_fvars (k n : ℕ) (x y : Fvar) (m : Term Fvar) :
   case lam ih => apply ih <;> aesop
   all_goals aesop
 
-variable [DecidableEq Fvar]
+variable [DecidableEq Var]
 
 /-- Substitution of a free variable not present in a term leaves it unchanged. -/
-theorem subst_fresh (x : Fvar) (t sub : Term Fvar) : x ∉ t.fv → (t [x := sub]) = t := by
+theorem subst_fresh (x : Var) (t sub : Term Var) : x ∉ t.fv → (t [x := sub]) = t := by
   induction t <;> intros <;> aesop
 
 /- Opening and closing are inverses. -/
-lemma open_close (x : Fvar) (t : Term Fvar) (k : ℕ) : x ∉ t.fv → t⟦k ↝ fvar x⟧⟦k ↜ x⟧ = t := by
+lemma open_close (x : Var) (t : Term Var) (k : ℕ) : x ∉ t.fv → t⟦k ↝ fvar x⟧⟦k ↜ x⟧ = t := by
   intros mem
   revert k
   induction t <;> intros k <;> simp
@@ -48,13 +48,13 @@ lemma open_close (x : Fvar) (t : Term Fvar) (k : ℕ) : x ∉ t.fv → t⟦k ↝
   all_goals aesop
 
 /-- Opening is injective. -/
-lemma open_injective (x : Fvar) (M M' : Term Fvar) : x ∉ M.fv → x ∉ M'.fv → M ^ fvar x = M' ^ fvar x → M = M' := by
+lemma open_injective (x : Var) (M M' : Term Var) : x ∉ M.fv → x ∉ M'.fv → M ^ fvar x = M' ^ fvar x → M = M' := by
   intros free_M free_M' eq
   rw [←open_close x M 0 free_M, ←open_close x M' 0 free_M']
   exact congrArg (close_rec 0 x) eq
 
 /-- Opening and closing are associative for nonclashing free variables. -/
-lemma swap_open_fvar_close (k n: ℕ) (x y : Fvar) (m : Term Fvar) : 
+lemma swap_open_fvar_close (k n: ℕ) (x y : Var) (m : Term Var) : 
     k ≠ n → x ≠ y → m⟦n ↝ fvar y⟧⟦k ↜ x⟧ = m⟦k ↜ x⟧⟦n ↝ fvar y⟧ := by
   revert k n
   induction' m <;> intros k n ne_kn ne_xy <;> simp
@@ -64,7 +64,7 @@ lemma swap_open_fvar_close (k n: ℕ) (x y : Fvar) (m : Term Fvar) :
   all_goals aesop
 
 /-- Closing preserves free variables. -/
-lemma close_preserve_not_fvar {k x y} (m : Term Fvar) : x ∉ m.fv → x ∉ (m⟦k ↜ y⟧).fv := by
+lemma close_preserve_not_fvar {k x y} (m : Term Var) : x ∉ m.fv → x ∉ (m⟦k ↜ y⟧).fv := by
   intros mem
   revert k
   induction m <;> intros k <;> simp
@@ -73,7 +73,7 @@ lemma close_preserve_not_fvar {k x y} (m : Term Fvar) : x ∉ m.fv → x ∉ (m�
   all_goals aesop
 
 /-- Opening to a fresh free variable preserves free variables. -/
-lemma open_fresh_preserve_not_fvar {k x y} (m : Term Fvar) : x ∉ m.fv → x ≠ y → x ∉ (m⟦k ↝ fvar y⟧).fv := by
+lemma open_fresh_preserve_not_fvar {k x y} (m : Term Var) : x ∉ m.fv → x ≠ y → x ∉ (m⟦k ↝ fvar y⟧).fv := by
   intros mem neq
   revert k
   induction m <;> intros k <;> simp
@@ -83,7 +83,7 @@ lemma open_fresh_preserve_not_fvar {k x y} (m : Term Fvar) : x ∉ m.fv → x �
   all_goals aesop
 
 /-- Substitution preserves free variables. -/
-lemma subst_preserve_not_fvar {x y} (m n : Term Fvar) : x ∉ m.fv ∪ n.fv → x ∉ (m [y := n]).fv := by
+lemma subst_preserve_not_fvar {x y} (m n : Term Var) : x ∉ m.fv ∪ n.fv → x ∉ (m [y := n]).fv := by
   intros mem
   simp at mem
   induction m <;> simp
@@ -92,7 +92,7 @@ lemma subst_preserve_not_fvar {x y} (m n : Term Fvar) : x ∉ m.fv ∪ n.fv → 
   all_goals aesop
 
 /-- Closing removes a free variable. -/
-lemma close_var_not_fvar_rec (x) (k) (t : Term Fvar) : x ∉ (t⟦k ↜ x⟧).fv := by
+lemma close_var_not_fvar_rec (x) (k) (t : Term Var) : x ∉ (t⟦k ↜ x⟧).fv := by
   revert k
   induction t <;> intros k <;> simp
   case fvar x' => split <;> simp_all
@@ -100,13 +100,13 @@ lemma close_var_not_fvar_rec (x) (k) (t : Term Fvar) : x ∉ (t⟦k ↜ x⟧).fv
   all_goals aesop
 
 /-- Specializes `close_var_not_fvar_rec` to first closing. -/
-lemma close_var_not_fvar (x) (t : Term Fvar) : x ∉ (t ^* x).fv := close_var_not_fvar_rec x 0 t
+lemma close_var_not_fvar (x) (t : Term Var) : x ∉ (t ^* x).fv := close_var_not_fvar_rec x 0 t
 
-variable [HasFresh Fvar] 
+variable [HasFresh Var] 
 
-omit [DecidableEq Fvar] in
+omit [DecidableEq Var] in
 /-- A locally closed term is unchanged by opening. -/
-lemma open_lc (k t) (e : Term Fvar) : e.LC → e = e⟦k ↝ t⟧ := by
+lemma open_lc (k t) (e : Term Var) : e.LC → e = e⟦k ↝ t⟧ := by
   intros e_lc
   revert k
   induction e_lc <;> intros k <;> simp
@@ -114,7 +114,7 @@ lemma open_lc (k t) (e : Term Fvar) : e.LC → e = e⟦k ↝ t⟧ := by
   case lam xs e _ ih => refine open_lc_aux e 0 (fvar (fresh xs)) (k+1) t ?_ ?_ <;> aesop
 
 /-- Substitution of a locally closed term distributes with opening. -/
-lemma subst_open (x : Fvar) (t : Term Fvar) (k : ℕ) (u e) :
+lemma subst_open (x : Var) (t : Term Var) (k : ℕ) (u e) :
   LC t → 
   (e ⟦ k ↝ u ⟧) [ x := t ] = (e [ x := t ]) ⟦k ↝  u [ x := t ]⟧ := by
   revert k
@@ -127,12 +127,12 @@ lemma subst_open (x : Fvar) (t : Term Fvar) (k : ℕ) (u e) :
   case app ih_l ih_r => exact ⟨ih_l k t_lv, ih_r k t_lv⟩
 
 /-- Specialize `subst_open` to the first opening. -/
-theorem subst_open_var (x y : Fvar) (u e : Term Fvar) : y ≠ x → LC u → (e [y := u]) ^ fvar x = (e ^ fvar x) [y := u] := by
+theorem subst_open_var (x y : Var) (u e : Term Var) : y ≠ x → LC u → (e [y := u]) ^ fvar x = (e ^ fvar x) [y := u] := by
   intros neq u_lc
   simp [neq, subst_open y u 0 (fvar x) e u_lc]
 
 /-- Substitution of locally closed terms is locally closed. -/
-theorem subst_lc {x : Fvar} {e u : Term Fvar} : LC e → LC u → LC (e [x := u]) := by
+theorem subst_lc {x : Var} {e u : Term Var} : LC e → LC u → LC (e [x := u]) := by
   intros lc_e lc_u
   induction lc_e <;> simp
   case fvar => split <;> [assumption; constructor] 
@@ -145,7 +145,7 @@ theorem subst_lc {x : Fvar} {e u : Term Fvar} : LC e → LC u → LC (e [x := u]
     all_goals aesop
 
 /-- Opening to a term `t` is equivalent to opening to a free variable and substituting it for `t`. -/
-lemma subst_intro (x : Fvar) (t e : Term Fvar) : x ∉ e.fv → LC t → e ^ t = (e ^ fvar x) [ x := t ] := by
+lemma subst_intro (x : Var) (t e : Term Var) : x ∉ e.fv → LC t → e ^ t = (e ^ fvar x) [ x := t ] := by
   intros mem t_lc
   simp [open']
   rw [subst_open x t 0 (fvar x) e t_lc]
@@ -154,7 +154,7 @@ lemma subst_intro (x : Fvar) (t e : Term Fvar) : x ∉ e.fv → LC t → e ^ t =
   exact mem
 
 /-- Opening of locally closed terms is locally closed. -/
-theorem beta_lc {M N : Term Fvar} : LC (lam M) → LC N → LC (M ^ N) := by
+theorem beta_lc {M N : Term Var} : LC (lam M) → LC N → LC (M ^ N) := by
   intros m_lc
   cases m_lc
   case lam xs mem =>
@@ -168,7 +168,7 @@ theorem beta_lc {M N : Term Fvar} : LC (lam M) → LC N → LC (M ^ N) := by
     all_goals aesop        
 
 /-- Opening then closing is equivalent to substitution. -/
-lemma open_close_to_subst (m : Term Fvar) (x y : Fvar) (k : ℕ) : LC m → m ⟦k ↜ x⟧⟦k ↝ fvar y⟧ = m [x := fvar y] := by
+lemma open_close_to_subst (m : Term Var) (x y : Var) (k : ℕ) : LC m → m ⟦k ↜ x⟧⟦k ↝ fvar y⟧ = m [x := fvar y] := by
   intros m_lc
   revert k
   induction' m_lc <;> intros k <;> simp
@@ -190,7 +190,7 @@ lemma open_close_to_subst (m : Term Fvar) (x y : Fvar) (k : ℕ) : LC m → m �
     all_goals aesop
 
 /-- Closing and opening are inverses. -/
-lemma close_open (x : Fvar) (t : Term Fvar) (k : ℕ) : LC t → t⟦k ↜ x⟧⟦k ↝ fvar x⟧ = t := by
+lemma close_open (x : Var) (t : Term Var) (k : ℕ) : LC t → t⟦k ↜ x⟧⟦k ↝ fvar x⟧ = t := by
   intros lc_t
   revert k
   induction lc_t <;> intros k <;> simp
